Work on Topological Order

Properties.thy
@@ -1,5 +1,5 @@
 theory Properties
-  imports blockDAG Extend_blockDAG Spectre Ghostdag
+  imports blockDAG Extend_blockDAG 
 begin
 
 definition Linear_Order:: "(('a,'b) pre_digraph \<Rightarrow> 'a rel) \<Rightarrow> bool"
@@ -10,12 +10,13 @@ definition Order_Preserving:: "(('a,'b) pre_digraph \<Rightarrow> 'a rel) \<Righ
   where "Order_Preserving A \<equiv> (\<forall>G a b. blockDAG G \<longrightarrow> a \<rightarrow>\<^sup>+\<^bsub>G\<^esub> b \<longrightarrow> (b,a) \<in> (A G))"
 
 
-definition One_Appending_Monotone:: "(('a,'b) pre_digraph \<Rightarrow> 'a rel) \<Rightarrow> bool "
-  where "One_Appending_Monotone A \<equiv>
+definition Honest_One_Appending_Monotone:: "(('a,'b) pre_digraph \<Rightarrow> 'a rel) \<Rightarrow> bool "
+  where "Honest_One_Appending_Monotone A \<equiv>
          (\<forall>G G_A a b c. Honest_Append_One G G_A a \<longrightarrow> ((b,c) \<in> (A G) \<longrightarrow> (b,c) \<in> (A G_A)))"
 
-definition One_Appending_Monotone2:: "(('a,'b) pre_digraph \<Rightarrow> 'a rel) \<Rightarrow> bool "
-  where "One_Appending_Monotone2 A \<equiv>
+
+definition One_Appending_Monotone:: "(('a,'b) pre_digraph \<Rightarrow> 'a rel) \<Rightarrow> bool "
+  where "One_Appending_Monotone A \<equiv>
          (\<forall>G G_A a b c. (Append_One G G_A a 
         \<and> ((b \<in> past_nodes G_A a \<and> c \<in> past_nodes G_A a)
         \<or> (b \<notin> past_nodes G_A a \<and> c \<notin> past_nodes G_A a)))
