Verts_To_List.thy
@@ -1,0 +1,86 @@
+theory Verts_To_List
+  imports Utils  "HOL-Library.Comparator" Extend_blockDAG
+begin
+
+
+text \<open>Function to sort a list $L$ under a graph G such if $a$ references $b$,
+$b$ precedes $a$ in the list\<close>
+
+fun unfold_referencing_verts:: "('a::linorder,'b) pre_digraph \<Rightarrow> 'a \<Rightarrow> 'a list" 
+  where "unfold_referencing_verts G a = sorted_list_of_set ({b \<in> verts G. dominates G b a} \<union> {a})"  
+
+
+fun unfold_referencing_verts_ex:: "('a::linorder,'b) pre_digraph \<Rightarrow> 'a \<Rightarrow> 'a list" 
+  where "unfold_referencing_verts_ex G a = sorted_list_of_set ({b \<in> verts G. dominates G b a})"  
+
+fun Verts_To_List_Rec:: "('a::linorder,'b) pre_digraph \<Rightarrow> 'a list \<Rightarrow> nat \<Rightarrow> 'a list"
+  where "Verts_To_List_Rec G L c = (if (c \<le> 0)
+  then L else Verts_To_List_Rec G (foldr (@) (map (unfold_referencing_verts G) L) []) (c - 1))"
+ 
+fun Verts_To_List:: "('a::linorder,'b) pre_digraph \<Rightarrow> 'a list"
+  where "Verts_To_List G = remdups (Verts_To_List_Rec G [genesis_nodeAlt G] 
+  (card (arcs G)))"
+
+function Depth_first_search_rec:: "('a::linorder,'b) pre_digraph \<Rightarrow> 'a \<Rightarrow> 'a list"
+  where "Depth_first_search_rec G a  = 
+ (if(\<not> DAG G) then [] else (foldr (@) 
+  (map (Depth_first_search_rec G) (unfold_referencing_verts_ex G a)) []) @ [a])"
+  by auto
+termination
+proof
+  let ?R = " measure ( \<lambda>(G, a). card {e \<in> verts G. e \<rightarrow>\<^sup>+\<^bsub>G\<^esub> a})"  
+  show "wf ?R"
+    by simp 
+next
+  fix G::"('a::linorder,'b) pre_digraph"
+  and a x::'a 
+  assume "\<not> \<not> DAG G" 
+  then interpret D: DAG G by auto
+  assume x_in: "x \<in> set (unfold_referencing_verts_ex G a)"
+  then have ff: "finite {b \<in> verts G. b \<rightarrow>\<^bsub>G\<^esub> a}" using D.finite_verts
+    by simp 
+  then have xa: "x \<rightarrow>\<^sup>+\<^bsub>G\<^esub> a" using x_in unfolding unfold_referencing_verts_ex.simps 
+    using sorted_list_of_set(1)
+    by auto 
+  then have "\<And>b. b \<rightarrow>\<^sup>+\<^bsub>G\<^esub> x \<Longrightarrow>  b \<rightarrow>\<^sup>+\<^bsub>G\<^esub> a" using trancl_trans by auto
+  then have "{b \<in> verts G.  b \<rightarrow>\<^sup>+\<^bsub>G\<^esub> x} \<subseteq> {b \<in> verts G.  b \<rightarrow>\<^sup>+\<^bsub>G\<^esub> a}"
+    by blast
+  moreover have "\<not> x \<rightarrow>\<^sup>+\<^bsub>G\<^esub> x" using D.cycle_free by simp
+  ultimately have "{b \<in> verts G.  b \<rightarrow>\<^sup>+\<^bsub>G\<^esub> x} \<subset> {b \<in> verts G.  b \<rightarrow>\<^sup>+\<^bsub>G\<^esub> a}" 
+    using xa D.reachable1_in_verts(1) by blast 
+  then have "card {b \<in> verts G.  b \<rightarrow>\<^sup>+\<^bsub>G\<^esub> x} < card {b \<in> verts G.  b \<rightarrow>\<^sup>+\<^bsub>G\<^esub> a}"
+    by (simp add: psubset_card_mono)
+  then show "((G, x), G, a) \<in> measure (\<lambda>(G, a). card {e \<in> verts G. e \<rightarrow>\<^sup>+\<^bsub>G\<^esub> a})"
+    by simp
+qed
+
+
+fun Depth_first_search_a:: "('a::linorder,'b) pre_digraph \<Rightarrow> 'a \<Rightarrow> 'a list"
+  where "Depth_first_search_a G a =  rev (remdups (Depth_first_search_rec G a))"
+
+fun Depth_first_search:: "('a::linorder,'b) pre_digraph \<Rightarrow> 'a list"
+  where "Depth_first_search G =  Depth_first_search_a G (genesis_nodeAlt G)"
+
+lemma Depth_first_search_sub:
+  fixes G::"('a::linorder, 'b) pre_digraph"
+shows "set (Depth_first_search G) \<subseteq> verts G"
+  unfolding Depth_first_search.simps  Depth_first_search_a.simps
+sorry
+
+
+lemma Depth_first_search_top:
+  assumes "blockDAG G" 
+  and "b \<rightarrow>\<^sup>+\<^bsub>G\<^esub> a"
+shows "(a,b) \<in> list_to_rel (Depth_first_search G)"
+  using assms(1,2)
+proof(induct G rule: blockDAG_induct_append)
+  case (base V)
+  then interpret bV: blockDAG V by auto
+  have False using base(2) 
+    unfolding arcs_ends_def bV.gen_graph_empty_arcs arc_to_ends_def by force
+  then show ?case by auto
+next
+  case (step H)
+  then show ?case sorry
+qed
+end
